## Properties of the Binomial Coefficients

1. __Expansion__:  

$$
{n \choose k}=
\begin{cases}
\frac{n!}{k!(n-k)!}=\frac{n^{\underline{k}}}{k!}=\frac{P(n,k}{k!} \quad if \;0 \leq k \leq n, \\
0 \quad otherwise
\end{cases}
 $$

2. ${n \choose k}={n \choose n-k}$

3. ${n \choose k}={n-1 \choose k}+{n-1 \choose k-1}$

4. __Binomial Theorem:__
$$(x+y)^n=\sum_{k=0}^n {n \choose k}x^ky^{n-k}$$

5. $\sum_{k=0}^n{n \choose k}=2^n$, when $x=1 \;and\;y=1$

6. Summing over lower index (or symmetry. Accross row $n$ of Pascal's Triangle):
$$\sum_{k}(-1)^k{n \choose k}=
\begin{cases}
0 \;if\;n\geq1 \\
1 \;if\;n=0 
\end{cases}
$$

7. Summing over upper index (i.e. summing by column in Pascal's Triangle):
$$\sum_{k=0}^n{k \choose m}={n+1 \choose m+1}$$
with $m$ being the column index, and $n$ being the row. After summing, we have a sum of all values in column $m$, from row $0$ to row $n$.

8. Vandermonde's identity:
$${m+n \choose r}=\sum_{k}{m \choose k}{n \choose r-k}$$

Intuitive explanation: Suppose a group has $m$ males and $n$ females. The number of ways to pick a smaller group of $r$ members, in which there are $k$ males and $r-k$ females is:

- When picking directly from the original group of $m+n$ people, we have: ${m+n \choose r}$
- When picking $k$ males from $m$ males and $r-k$ females from $n$ females, we have: $\sum{m \choose k}{n \choose r-k}$

## Exercises

### Ex 1

Combinatorial proof that $\sum {n \choose k}=2^n \; (*)$:

We have: 
- When n=0,
$$\sum{n \choose k}=2^0=1$$
So $(*)$ is true.

- When n>0, suppose that:
$$\sum_{k=0}^j{j \choose k}=2^j$$
with j being a positive integer.
We need to prove that: 
$$\sum_{k=0}^{j+1}{j+1 \choose k}=2^j+1$$
If this is true, then by induction, the identity holds for all non-negative $n$.

- We have:
$${j+1 \choose k}={j \choose k}+{j \choose k-1}$$
So:
$$\sum{j+1 \choose k}=\sum{j \choose k}+\sum{j \choose k-1}=2^J+2^J=2^{j+1}$$

### Ex 2

Prove the absorption/extraction identity: If $n$ is a positive integer and $k$ is a nonzero integer, then:

$${n \choose k}=\frac{n}{k}{n-1 \choose k-1} \quad (*)$$

---
We have the RHS of $(*)$ can be transformed as:

$$\frac{n}{k}\cdot\frac{(n-1)!}{(k-1)!(n-1-k+1)!}=\frac{n!}{(n-k)!}=LHS$$

---
### Ex 3

> Use algebraic methods to prove the cancellation identity: If $n$ and $k$ are nonnegative integers and $m$ is an integer with $m\leq n$, then:
$${n \choose k}{k \choose m}={n \choose m}{m-n \choose k-m}$$

We have: 

$$\begin{aligned}
RHS &= \frac{n!}{k!(n-k)!}\frac{k!}{m!(k-m)!} \\
&= \frac{}{}
\end{aligned}
$$

